Examples/List_Interface.thy
@@ -1,0 +1,40 @@
+theory List_Interface
+imports "../Refine_Imperative_HOL/Sepref"
+begin
+
+section "List Interface"
+
+
+context
+  fixes n::nat
+begin
+  definition "mop_empty_list = SPECT [ [] \<mapsto> enat n ]"
+
+  sepref_register "mop_empty_list" 
+  print_theorems 
+end
+
+context
+  fixes t::"'a list \<Rightarrow>nat"
+begin
+  definition "mop_push_list  x xs = SPECT [ ( xs @ [x] ) \<mapsto> enat (t xs) ]"
+  
+  sepref_register "mop_push_list" 
+  print_theorems
+  thm   mop_push_list.pat
+end
+
+
+context
+  fixes n::nat
+begin
+  definition "mop_lookup_list xs i = SPECT [ xs ! i \<mapsto> enat n ]"
+
+  sepref_register "mop_lookup_list" 
+  print_theorems 
+end
+
+
+
+
+end
